%2multibyte Version: 5.50.0.2960 CodePage: 1252

\documentclass{article}
%%%%%%%%%%%%%%%%%%%%%%%%%%%%%%%%%%%%%%%%%%%%%%%%%%%%%%%%%%%%%%%%%%%%%%%%%%%%%%%%%%%%%%%%%%%%%%%%%%%%%%%%%%%%%%%%%%%%%%%%%%%%%%%%%%%%%%%%%%%%%%%%%%%%%%%%%%%%%%%%%%%%%%%%%%%%%%%%%%%%%%%%%%%%%%%%%%%%%%%%%%%%%%%%%%%%%%%%%%%%%%%%%%%%%%%%%%%%%%%%%%%%%%%%%%%%
%TCIDATA{OutputFilter=LATEX.DLL}
%TCIDATA{Version=5.50.0.2960}
%TCIDATA{Codepage=1252}
%TCIDATA{<META NAME="SaveForMode" CONTENT="1">}
%TCIDATA{BibliographyScheme=Manual}
%TCIDATA{Created=Wednesday, October 28, 2015 14:56:20}
%TCIDATA{LastRevised=Wednesday, October 28, 2015 15:38:44}
%TCIDATA{<META NAME="GraphicsSave" CONTENT="32">}
%TCIDATA{<META NAME="DocumentShell" CONTENT="Standard LaTeX\Blank - Standard LaTeX Article">}
%TCIDATA{CSTFile=40 LaTeX article.cst}

\newtheorem{theorem}{Theorem}
\newtheorem{acknowledgement}[theorem]{Acknowledgement}
\newtheorem{algorithm}[theorem]{Algorithm}
\newtheorem{axiom}[theorem]{Axiom}
\newtheorem{case}[theorem]{Case}
\newtheorem{claim}[theorem]{Claim}
\newtheorem{conclusion}[theorem]{Conclusion}
\newtheorem{condition}[theorem]{Condition}
\newtheorem{conjecture}[theorem]{Conjecture}
\newtheorem{corollary}[theorem]{Corollary}
\newtheorem{criterion}[theorem]{Criterion}
\newtheorem{definition}[theorem]{Definition}
\newtheorem{example}[theorem]{Example}
\newtheorem{exercise}[theorem]{Exercise}
\newtheorem{lemma}[theorem]{Lemma}
\newtheorem{notation}[theorem]{Notation}
\newtheorem{problem}[theorem]{Problem}
\newtheorem{proposition}[theorem]{Proposition}
\newtheorem{remark}[theorem]{Remark}
\newtheorem{solution}[theorem]{Solution}
\newtheorem{summary}[theorem]{Summary}
\newenvironment{proof}[1][Proof]{\noindent\textbf{#1.} }{\ \rule{0.5em}{0.5em}}
\input{tcilatex}

\begin{document}


\[
1=\beta R
\]

\[
cL^{\eta -1}=w
\]

\[
\alpha \frac{k^{\alpha -1}L^{1-\alpha }}{X}=r_{k}
\]

\[
R=r_{k}+1-\delta 
\]

\[
\frac{\left( 1-\alpha \right) k^{\alpha }L^{-\alpha }}{X}=w
\]

\[
c+\delta k=k^{\alpha }L^{1-\alpha }
\]

\bigskip 

\bigskip 
\[
R=\frac{1}{\beta }
\]

\[
\frac{\left( 1-\alpha \right) k^{\alpha }L^{-\alpha }}{X}=\left( k^{\alpha
}L^{1-\alpha }-\delta k\right) L^{\eta -1}
\]

\begin{eqnarray*}
\alpha \frac{k^{\alpha -1}L^{1-\alpha }}{X} &=&\frac{1}{\beta }-1+\delta  \\
k &=&\left[ \frac{X}{\alpha }\left( \frac{1}{\beta }-1+\delta \right) \right]
^{\frac{1}{\alpha -1}}L
\end{eqnarray*}

\[
L^{1-\alpha }=\frac{X}{\alpha }\left( \frac{1}{\beta }-1+\delta \right)
k^{1-\alpha }
\]

\bigskip 

\begin{eqnarray*}
\frac{\left( 1-\alpha \right) }{X}\left( \frac{k}{L}\right) ^{\alpha }
&=&\left( \frac{X}{\alpha }\left( \frac{1}{\beta }-1+\delta \right) -\delta
\right) kL^{\eta -1} \\
\frac{\left( 1-\alpha \right) }{X}\left[ \frac{X}{\alpha }\left( \frac{1}{%
\beta }-1+\delta \right) \right] ^{\frac{\alpha }{\alpha -1}} &=&\left( 
\frac{X}{\alpha }\left( \frac{1}{\beta }-1+\delta \right) -\delta \right) %
\left[ \frac{X}{\alpha }\left( \frac{1}{\beta }-1+\delta \right) \right] ^{%
\frac{1}{\alpha -1}}L^{\eta } \\
L^{\eta } &=&\frac{\frac{\left( 1-\alpha \right) }{X}\left[ \frac{X}{\alpha }%
\left( \frac{1}{\beta }-1+\delta \right) \right] ^{\frac{\alpha }{\alpha -1}}%
}{\left( \frac{X}{\alpha }\left( \frac{1}{\beta }-1+\delta \right) -\delta
\right) \left[ \frac{X}{\alpha }\left( \frac{1}{\beta }-1+\delta \right) %
\right] ^{\frac{1}{\alpha -1}}}
\end{eqnarray*}

\end{document}
